src/CertifiedExtraction/Extraction/Refactor/Decompose.v
@@ -59,5 +59,71 @@ Definition DecomposeIndexedQueryStructurePre av qs_schema Index
            (r : IndexedQueryStructure qs_schema Index) :=
   DecomposePrei3list _ _ rWrap r.
 
+Definition DecomposeRep_well_behaved
+           av {n n' : nat}
+           {consSigs : Vector.t consSig n}
+           {methSigs : Vector.t methSig n'}
+           (adt : DecoratedADT (BuildADTSig consSigs methSigs))
+           (DecomposeRep : Rep adt -> list (Value av)) :=
+  forall x x0 : Rep adt,
+    is_same_types (DecomposeRep x0)
+                  (DecomposeRep x) = true.
+
 Arguments DecomposeIndexedQueryStructurePost _ _ _ _ _ _ / .
 Arguments DecomposeIndexedQueryStructurePre _ _ _ _ _ / .
+
+Definition coDomainWrappers
+           av {n n' : nat}
+           {consSigs : Vector.t consSig n}
+           {methSigs : Vector.t methSig n'}
+           (adt : DecoratedADT (BuildADTSig consSigs methSigs))
+  := forall midx : Fin.t n', CodWrapperT av (methCod (Vector.nth methSigs midx)).
+
+Definition domainWrappers
+           av {n n' : nat}
+           {consSigs : Vector.t consSig n}
+           {methSigs : Vector.t methSig n'}
+           (adt : DecoratedADT (BuildADTSig consSigs methSigs))
+  := forall midx : Fin.t n', DomWrapperT av (methDom (Vector.nth methSigs midx)).
+
+Definition DecomposeIndexedQueryStructure' av qs_schema Index
+           (rWrap : @RepWrapperT av (QueryStructureSchema.numRawQSschemaSchemas qs_schema)
+                                 Schema.RawSchema
+                                 (fun ns : Schema.RawSchema =>
+                                    SearchUpdateTerms (Schema.rawSchemaHeading ns))
+                                 (fun (ns : Schema.RawSchema)
+                                      (_ : SearchUpdateTerms (Schema.rawSchemaHeading ns)) =>
+                                    @IndexedEnsembles.IndexedEnsemble
+                                      (@RawTuple (Schema.rawSchemaHeading ns)))
+                                 (QueryStructureSchema.qschemaSchemas qs_schema) Index)
+
+           (r : IndexedQueryStructure qs_schema Index) :=
+  Decomposei3list _ _ rWrap (id r).
+
+Definition DecomposeIndexedQueryStructurePost' av qs_schema Index
+           (rWrap : @RepWrapperT av (QueryStructureSchema.numRawQSschemaSchemas qs_schema)
+                                 Schema.RawSchema
+                                 (fun ns : Schema.RawSchema =>
+                                    SearchUpdateTerms (Schema.rawSchemaHeading ns))
+                                 (fun (ns : Schema.RawSchema)
+                                      (_ : SearchUpdateTerms (Schema.rawSchemaHeading ns)) =>
+                                    @IndexedEnsembles.IndexedEnsemble
+                                      (@RawTuple (Schema.rawSchemaHeading ns)))
+                                 (QueryStructureSchema.qschemaSchemas qs_schema) Index)
+
+           (r r' : IndexedQueryStructure qs_schema Index) :=
+  DecomposePosti3list _ _ rWrap (id r) (id r').
+
+Definition DecomposeIndexedQueryStructurePre' av qs_schema Index
+           (rWrap : @RepWrapperT av (QueryStructureSchema.numRawQSschemaSchemas qs_schema)
+                                 Schema.RawSchema
+                                 (fun ns : Schema.RawSchema =>
+                                    SearchUpdateTerms (Schema.rawSchemaHeading ns))
+                                 (fun (ns : Schema.RawSchema)
+                                      (_ : SearchUpdateTerms (Schema.rawSchemaHeading ns)) =>
+                                    @IndexedEnsembles.IndexedEnsemble
+                                      (@RawTuple (Schema.rawSchemaHeading ns)))
+                                 (QueryStructureSchema.qschemaSchemas qs_schema) Index)
+
+           (r : IndexedQueryStructure qs_schema Index) :=
+  DecomposePrei3list _ _ rWrap (id r).
